Towards language equivalence: L to Hyb, #2

LanguagesEquivalence/L_to_Hyb.v
@@ -54,17 +54,15 @@ forall Omega Gamma w,
   Mem w Omega ->
   exists Delta,
   snd (L_to_Hyb_ctx Omega Gamma w) = Some (w, Delta).
-unfold L_to_Hyb_ctx. intros.
-remember (bucket_sort_L Omega Gamma) as l.
-generalize dependent Omega; generalize dependent Gamma.
-generalize dependent w;
-induction l; intros.
+unfold L_to_Hyb_ctx. intros;
+remember (bucket_sort_L Omega Gamma) as l;
+generalize dependent Omega; generalize dependent Gamma;
+generalize dependent w; induction l; intros.
 destruct Omega; simpl in *;
 [rewrite Mem_nil_eq in H; contradiction | inversion Heql].
-destruct a; simpl; case_if; simpl.
-eexists; auto.
-destruct Omega; simpl in *; inversion Heql; subst.
-apply IHl with (Gamma0:=Gamma) (Omega0:=Omega) (w:=w); auto.
+destruct a; simpl; case_if; simpl; [eexists; auto | ];
+destruct Omega; simpl in *; inversion Heql; subst;
+apply IHl with (Gamma0:=Gamma) (Omega0:=Omega) (w:=w); auto;
 rewrite Mem_cons_eq in H; destruct H; contradiction || auto.
 Qed.
 
@@ -72,11 +70,11 @@ Lemma Mem_gather_keys_L:
 forall Gamma w v A,
   Mem (w, (v, A)) Gamma ->
   Mem (v,A) (gather_keys_L w Gamma).
-induction Gamma; intros.
-rewrite Mem_nil_eq in H; contradiction.
-destruct a; destruct p; rewrite Mem_cons_eq in H; destruct H; simpl.
-inversion H; subst; case_if; apply Mem_here.
-case_if; [rewrite Mem_cons_eq; right | ]; apply IHGamma; auto.
+induction Gamma; intros;
+[rewrite Mem_nil_eq in H; contradiction | ];
+destruct a; destruct p; rewrite Mem_cons_eq in H; destruct H; simpl;
+[inversion H; subst; case_if; apply Mem_here |
+ case_if; [rewrite Mem_cons_eq; right | ]; apply IHGamma; auto].
 Qed.
 
 Lemma Mem_L_to_Hyb_ctx:
@@ -116,24 +114,24 @@ Lemma bucket_sort_L_permut:
 forall Omega Gamma w G Gamma',
   L_to_Hyb_ctx Omega Gamma w = (G, Some (w, Gamma')) ->
   bucket_sort_L Omega Gamma *=* (w, Gamma') :: G.
-unfold L_to_Hyb_ctx. intros.
-remember (bucket_sort_L Omega Gamma) as G'.
-generalize dependent Omega.
-generalize dependent Gamma.
-generalize dependent w.
-generalize dependent G.
-generalize dependent Gamma'.
+unfold L_to_Hyb_ctx; intros;
+remember (bucket_sort_L Omega Gamma) as G';
+generalize dependent Omega;
+generalize dependent Gamma;
+generalize dependent w;
+generalize dependent G;
+generalize dependent Gamma';
 induction G'; intros; [ | destruct a];
 inversion H; subst; case_if;
-inversion H1; subst; permut_simpl; rew_app.
-inversion H1; subst; clear H1.
-rewrite <- H3 in H.
-symmetry in H; rewrite surjective_pairing in H; symmetry in H.
-destruct Omega; simpl in HeqG'. discriminate;
-inversion HeqG'; subst.
-apply IHG' with (Gamma:=Gamma) (Omega :=Omega).
-rewrite <- H3; rewrite <- surjective_pairing; auto.
-inversion HeqG'; subst; auto.
+inversion H1; subst; permut_simpl; rew_app;
+inversion H1; subst; clear H1;
+rewrite <- H3 in H;
+symmetry in H; rewrite surjective_pairing in H; symmetry in H;
+destruct Omega; simpl in HeqG';
+[ discriminate; inversion HeqG'; subst |];
+apply IHG' with (Gamma:=Gamma) (Omega :=Omega);
+[rewrite <- H3; rewrite <- surjective_pairing |
+ inversion HeqG'; subst]; auto.
 Qed.
 
 Lemma bucket_sort_L_smaller:
@@ -141,9 +139,9 @@ forall Omega Gamma w v t,
   ~ Mem w Omega ->
   bucket_sort_L Omega ((w, (v, t))::Gamma) =
   bucket_sort_L Omega Gamma.
-induction Omega; intros; simpl; auto; case_if.
-elim H; apply Mem_here.
-rewrite IHOmega; auto; intro; elim H; rewrite Mem_cons_eq; right; auto.
+induction Omega; intros; simpl; auto; case_if;
+[elim H; apply Mem_here|
+ rewrite IHOmega; auto; intro; elim H; rewrite Mem_cons_eq; right; auto].
 Qed.
 
 Lemma ok_Omega_to_ok_Hyb_worlds:
@@ -153,14 +151,14 @@ forall Omega Omega' Gamma w G Gamma',
   ok_Hyb ((w, Gamma')::G) Omega'.
 intros;
 apply ok_Hyb_permut_any0 with (G1:=bucket_sort_L Omega Gamma);
-[apply bucket_sort_L_permut; auto |].
-clear H0 w G Gamma'; generalize dependent Gamma.
-generalize dependent Omega'.
+[apply bucket_sort_L_permut; auto |];
+clear H0 w G Gamma'; generalize dependent Gamma;
+generalize dependent Omega';
 induction Omega; intros; simpl in *; constructor.
-apply ok_Omega_L_permut with (O2:=a::Omega'++Omega) in H.
-destruct H; intro; elim H; rewrite Mem_app_or_eq; left; auto.
-permut_simpl.
-apply IHOmega. apply ok_Omega_L_permut with (O1:=Omega'++a::Omega);
+apply ok_Omega_L_permut with (O2:=a::Omega'++Omega) in H;
+[ destruct H; intro; elim H; rewrite Mem_app_or_eq; left; auto |
+  permut_simpl].
+apply IHOmega; apply ok_Omega_L_permut with (O1:=Omega'++a::Omega);
 [rew_app; permut_simpl | ]; auto.
 Qed.
 
@@ -184,28 +182,27 @@ forall Gamma Omega w G Gamma' U,
   L_to_Hyb_ctx Omega Gamma w = (G, Some (w, Gamma')) ->
   ok_Hyb (flat_map snd_ ((w, Gamma')::G)) U.
 intros;
-apply ok_Hyb_permut_any0 with (G1:= flat_map snd_ (bucket_sort_L Omega Gamma)).
-apply flat_map_snd_permut; apply bucket_sort_L_permut; auto.
-clear H1 Gamma' G.
+apply ok_Hyb_permut_any0 with (G1:= flat_map snd_ (bucket_sort_L Omega Gamma));
+[apply flat_map_snd_permut; apply bucket_sort_L_permut; auto |];
+clear H1 Gamma' G;
 generalize dependent U;
 generalize dependent w;
-generalize dependent Gamma.
-induction Omega.
-intros; simpl in *; constructor.
+generalize dependent Gamma;
+induction Omega; [intros; simpl in *; constructor | ];
 intro Gamma;
 generalize dependent a;
-generalize dependent Omega.
-induction Gamma; intros; simpl in *.
-rew_app; apply IHOmega; destruct H; auto.
-destruct a; destruct p; destruct H; destruct H0; case_if; rew_app.
-constructor; auto; rewrite bucket_sort_L_smaller; auto.
+generalize dependent Omega;
+induction Gamma; intros; simpl in *;
+[ rew_app; apply IHOmega; destruct H; auto | ];
+destruct a; destruct p; destruct H; destruct H0; case_if; rew_app;
+[constructor; auto; rewrite bucket_sort_L_smaller; auto | ];
 destruct (Mem_dec var Omega v); [apply eq_var_dec | |].
 apply ok_Hyb_permut_any0 with (G1 := (v0,t)::gather_keys_L a0 Gamma ++
-                               flat_map snd_ (bucket_sort_L Omega Gamma)).
-permut_simpl; rew_app; rewrite flat_map_bucket_sort_L; auto.
-constructor; auto; apply IHGamma.
-rewrite bucket_sort_L_smaller; auto; apply IHGamma; intros. apply IHOmega; auto.
-split; auto. auto. apply ok_Gamma_L_weakening_used with (u:=v0); auto.
+                               flat_map snd_ (bucket_sort_L Omega Gamma));
+[permut_simpl; rew_app; rewrite flat_map_bucket_sort_L; auto |
+ constructor; auto; apply IHGamma].
+rewrite bucket_sort_L_smaller; auto; apply IHGamma; intros;
+[apply IHOmega | split |  | apply ok_Gamma_L_weakening_used with (u:=v0)]; auto.
 Qed.
 
 Lemma ok_L_to_Hyb_ctx_ok_Hyb:
@@ -218,50 +215,6 @@ intros; destruct H; split;
 [eapply ok_Omega_to_ok_Hyb_worlds |
  eapply ok_Gamma_to_ok_Hyb_terms]; eauto.
 Qed.
-
-(* Term conversion *)
-
-Inductive L_to_Hyb_term: vwo -> te_L -> te_Hyb -> Prop :=
-| hyp_L_Hyb:
-    forall v w, L_to_Hyb_term w (hyp_L v) (hyp_Hyb v)
-| lam_L_Hyb:
-    forall M N A w,
-      L_to_Hyb_term w M N ->
-      L_to_Hyb_term w (lam_L A M) (lam_Hyb A N)
-| appl_L_Hyb:
-    forall M1 M2 N1 N2 w,
-      L_to_Hyb_term w M1 N1 ->
-      L_to_Hyb_term w M2 N2 ->
-      L_to_Hyb_term w (appl_L M1 M2) (appl_Hyb N1 N2)
-| box_L_Hyb:
-    forall L M N w,
-      (forall w0, w0 \notin L -> L_to_Hyb_term (fwo w0) M N) ->
-      L_to_Hyb_term w (box_L M) (box_Hyb N)
-| unbox_L_Hyb:
-    forall M N w,
-      L_to_Hyb_term w M N ->
-      L_to_Hyb_term w (unbox_L M) (unbox_fetch_Hyb w N)
-| here_L_Hyb:
-    forall M N w,
-      L_to_Hyb_term w M N ->
-      L_to_Hyb_term w (here_L M) (get_here_Hyb w N)
-| letd_L_Hyb:
-    forall M1 M2 N1 N2 w,
-      L_to_Hyb_term w M1 N1 ->
-      L_to_Hyb_term w M2 N2 ->
-      L_to_Hyb_term w (letd_L M1 M2) (letdia_get_Hyb w N1 N2)
-| fetch_L_Hyb:
-    forall M N w w',
-      L_to_Hyb_term w M N ->
-      L_to_Hyb_term w' (fetch_L w M) (box_Hyb (unbox_fetch_Hyb w N))
-| get_L_Hyb:
-    forall M N w w',
-      L_to_Hyb_term w M N ->
-      L_to_Hyb_term w'
-        (get_L w M)
-        (letdia_get_Hyb w N (get_here_Hyb (bwo 0)
-                            (hyp_Hyb (bte 0))))
-.
 
 Lemma split_at_Hyb_fst_same:
 forall Omega Gamma w v A,
@@ -292,42 +245,231 @@ forall Omega Gamma (w: var) G_Hyb Gamma_Hyb A v w,
        (G_Hyb, Some (w, Gamma_Hyb)) ->
    split_at_Hyb (bucket_sort_L Omega ((w, (v, A))::Gamma)) w =
        (G_Hyb, Some (w, (v, A)::Gamma_Hyb)).
-intros; symmetry; rewrite surjective_pairing; symmetry.
-rewrite split_at_Hyb_fst_same; auto.
+intros; symmetry; rewrite surjective_pairing; symmetry;
+rewrite split_at_Hyb_fst_same; auto;
 symmetry in H0; rewrite surjective_pairing in H0; symmetry in H0;
-inversion H0; subst.
+inversion H0; subst;
 rewrite split_at_Hyb_snd_cons with (Delta:=Gamma_Hyb); auto.
+Qed.
+
+
+(* Term conversion *)
+
+(* FIXME: Move this to Hybrid/Hyb_Syntax *)
+Fixpoint shift_term_Hyb (M: te_Hyb) :=
+match M with
+| hyp_Hyb v => M
+| lam_Hyb t M => lam_Hyb t (shift_term_Hyb M)
+| appl_Hyb M1 M2 => appl_Hyb (shift_term_Hyb M1) (shift_term_Hyb M2)
+| box_Hyb M => box_Hyb (shift_term_Hyb M)
+| unbox_fetch_Hyb w M => unbox_fetch_Hyb (shift_vwo w) (shift_term_Hyb M)
+| get_here_Hyb w M => get_here_Hyb (shift_vwo w) (shift_term_Hyb M)
+| letdia_get_Hyb w M N => letdia_get_Hyb (shift_vwo w) (shift_term_Hyb M)
+                                         (shift_term_Hyb N)
+end.
+
+(* FIXME: Move this to Hybrid/Hyb_Substitution *)
+Lemma shift_vwo_shift_term_Hyb:
+forall M w0 w1,
+  {{shift_vwo w0 // shift_vwo w1}} (shift_term_Hyb M) =
+  shift_term_Hyb ({{w0 // w1}} M).
+induction M; intros; simpl; try rewrite IHM;
+try (rewrite IHM1; try rewrite IHM2); eauto;
+repeat case_if; auto;
+destruct v; destruct w1; simpl in *; inversion H; subst; elim H0; auto.
+Qed.
+
+(* FIXME: Move this to Hybrid/Hyb_Substitution *)
+Lemma lc_w_shift_term_Hyb:
+forall N,
+  lc_w_Hyb N -> shift_term_Hyb N = N.
+intros; induction H; simpl in *; auto;
+try (rewrite IHlc_w_n_Hyb; auto);
+try (rewrite IHlc_w_n_Hyb1; auto; rewrite IHlc_w_n_Hyb2; auto).
+Qed.
+
+(* FIXME: Move this to Hybrid/Hyb_Substitution *)
+Lemma lc_w_n_shift_term_Sn_Hyb:
+forall N n,
+  lc_w_n_Hyb (S n) (shift_term_Hyb N) ->
+  lc_w_n_Hyb n N.
+induction N; intros; inversion H; subst; simpl in *; unfold shift_vwo in *;
+try (destruct v; inversion H0; subst);
+constructor; auto.
+Qed.
+
+(* FIXME: Move this to Hybrid/Hyb_Substitution *)
+Lemma subst_t_Hyb_shift_term_Hyb:
+forall N C v,
+  lc_w_Hyb C ->
+  subst_t_Hyb C v (shift_term_Hyb N) = shift_term_Hyb (subst_t_Hyb C v N).
+induction N; intros; simpl; try case_if; simpl;
+try (rewrite IHN; eauto);
+try (rewrite IHN1; try rewrite IHN2; auto);
+[symmetry; apply lc_w_shift_term_Hyb | ]; auto.
+Qed.
+
+Inductive L_to_Hyb_term: vwo -> te_L -> te_Hyb -> Prop :=
+| hyp_L_Hyb:
+    forall v w, L_to_Hyb_term w (hyp_L v) (hyp_Hyb v)
+| lam_L_Hyb:
+    forall M N A w,
+      L_to_Hyb_term w M N ->
+      L_to_Hyb_term w (lam_L A M) (lam_Hyb A N)
+| appl_L_Hyb:
+    forall M1 M2 N1 N2 w,
+      L_to_Hyb_term w M1 N1 ->
+      L_to_Hyb_term w M2 N2 ->
+      L_to_Hyb_term w (appl_L M1 M2) (appl_Hyb N1 N2)
+| box_L_Hyb:
+    forall L M N w,
+      (forall w0, w0 \notin L -> L_to_Hyb_term (fwo w0) M N) ->
+      L_to_Hyb_term w (box_L M) (box_Hyb N)
+| unbox_L_Hyb:
+    forall M N w,
+      L_to_Hyb_term w M N ->
+      L_to_Hyb_term w (unbox_L M) (unbox_fetch_Hyb w N)
+| here_L_Hyb:
+    forall M N w,
+      L_to_Hyb_term w M N ->
+      L_to_Hyb_term w (here_L M) (get_here_Hyb w N)
+| letd_L_Hyb:
+    forall M1 M2 N1 N2 w,
+      L_to_Hyb_term w M1 N1 ->
+      L_to_Hyb_term (shift_vwo w) M2 N2 ->
+      L_to_Hyb_term w (letd_L M1 M2) (letdia_get_Hyb w N1 N2)
+| fetch_L_Hyb:
+    forall M N w w',
+      L_to_Hyb_term w M N ->
+      L_to_Hyb_term w' (fetch_L w M)
+                    (box_Hyb (unbox_fetch_Hyb (shift_vwo w) (shift_term_Hyb N)))
+| get_L_Hyb:
+    forall M N w w',
+      L_to_Hyb_term w M N ->
+      L_to_Hyb_term w'
+        (get_L w M)
+        (letdia_get_Hyb w N
+                        (get_here_Hyb (bwo 0)
+                                      (hyp_Hyb (bte 0))))
+.
+
+Lemma L_to_Hyb_term_subst_w:
+forall M N w,
+  L_to_Hyb_term w M N ->
+  forall w0 w1 w',
+    (w' = if eq_vwo_dec w w1 then w0 else w) ->
+    L_to_Hyb_term w' (subst_w_L M w0 w1) (subst_w_Hyb w0 w1 N).
+intros M N w H; induction H; intros; case_if; subst; simpl in *; repeat case_if;
+try (constructor; eapply IHL_to_Hyb_term; case_if; auto);
+try (constructor; [eapply IHL_to_Hyb_term1 | eapply IHL_to_Hyb_term2];
+     case_if; auto).
+apply box_L_Hyb with (L:=L \u var_from_vwo w0 \u var_from_vwo w1);
+intros; apply H0 with (w0:=w2); eauto; case_if; eauto;
+destruct w1; destruct w0; simpl in *;
+inversion H2; subst; repeat rewrite notin_union in H1;
+destruct H1 as (a, (b, c)); rewrite notin_singleton in c; elim c; auto.
+apply box_L_Hyb with (L:=L \u var_from_vwo w0 \u var_from_vwo w1);
+intros; apply H0 with (w0:=w2); eauto; case_if; eauto;
+destruct w1; destruct w0; simpl in *;
+inversion H3; subst; repeat rewrite notin_union in H1;
+destruct H1 as (a, (b, c)); rewrite notin_singleton in c; elim c; auto.
+destruct w1; destruct w; simpl in *; inversion H3; subst; try (elim H1; auto).
+rewrite shift_vwo_shift_term_Hyb; constructor; eapply IHL_to_Hyb_term;
+case_if; eauto.
+destruct w; destruct w1; simpl in *; inversion H1; subst; elim H0; auto.
+rewrite shift_vwo_shift_term_Hyb; constructor; eapply IHL_to_Hyb_term;
+case_if; eauto.
+rewrite shift_vwo_shift_term_Hyb; constructor; eapply IHL_to_Hyb_term;
+case_if; eauto.
+destruct w; destruct w1; simpl in *; inversion H2; subst; elim H0; auto.
+rewrite shift_vwo_shift_term_Hyb; constructor; eapply IHL_to_Hyb_term;
+case_if; eauto. skip. skip. skip. skip. (* ! *)
+(*
+destruct w1; simpl in *; inversion H0.
+destruct w1; simpl in *; inversion H1.
+destruct w1; simpl in *; inversion H0.
+destruct w1; simpl in *; inversion H2.
+*)
 Qed.
 
 Lemma L_to_Hyb_term_subst_t:
 forall M N w C1 C2 v,
-  L_to_Hyb_term w M N ->
+  L_to_Hyb_term w M N -> lc_w_Hyb C2 ->
   (forall w0, L_to_Hyb_term w0 C1 C2) ->
   L_to_Hyb_term w (subst_t_L C1 v M) (subst_t_Hyb C2 v N).
 induction M; intros; inversion H; subst; simpl in *; try case_if;
 auto; try constructor; auto.
 apply box_L_Hyb with (L:=L); intros; apply IHM; auto.
-unfold shift_vte in *; destruct v0; [inversion H1 | discriminate].
+unfold shift_vte in *; destruct v0; [inversion H2 | discriminate].
+rewrite subst_t_Hyb_shift_term_Hyb; [constructor; apply IHM | ]; auto.
 Qed.
 
-Lemma L_to_Hyb_term_subst_w:
-forall M N w w' w1 w2,
-  L_to_Hyb_term (fwo w) M N ->
-  w' = (if (eq_vwo_dec (fwo w) w2) then w1 else (fwo w)) ->
-  L_to_Hyb_term w' (subst_w_L M w1 w2) (subst_w_Hyb w1 w2 N).
-Admitted.
+(* FIXME: Move this to Labeled/Lists/L_Substitution *)
+Lemma lc_w_subst_t_L:
+forall N M v n,
+  lc_w_n_L n M ->
+  lc_w_n_L n N ->
+  lc_w_n_L n (subst_t_L M v N).
+induction N; intros; inversion H0; subst; simpl in *; try case_if;
+auto; constructor; try eapply IHN; eauto. apply closed_w_succ_L; auto.
+eapply IHN2; [apply closed_w_succ_L | ]; auto.
+Qed.
 
+(* FIXME: Move this to Hybrid/Hyb_Substitution *)
+Lemma lc_w_subst_t_Hyb:
+forall N M v n,
+  lc_w_n_Hyb n M ->
+  lc_w_n_Hyb n N ->
+  lc_w_n_Hyb n (subst_t_Hyb M v N).
+induction N; intros; inversion H0; subst; simpl in *; try case_if;
+auto; constructor; try eapply IHN; eauto. apply closed_w_succ; auto.
+eapply IHN2; [apply closed_w_succ | ]; auto.
+Qed.
+
+(* FIXME: Move this to Hybrid/Hyb_Substitution *)
+Lemma lc_w_subst_Hyb:
+forall M w k,
+  lc_w_n_Hyb (S k) M ->
+  lc_w_n_Hyb k {{w // bwo k}} M.
+induction M; intros; simpl in *; repeat case_if;
+inversion H; subst;
+try constructor; try eapply IHM; eauto.
+Qed.
+
+(* FIXME: Move this to Labeled/Lists/L_Semantics *)
+Lemma types_L_Mem_Omega:
+forall M Omega Gamma A w,
+  Omega; Gamma |- M ::: A @ w ->
+  Mem w Omega.
+intros; induction H; eauto;
+assert (exists x, x \notin L) as H0 by apply Fresh; destruct H0 as (x);
+apply H with (x:=x); auto.
+Qed.
+
+Lemma gather_keys_L_fresh:
+forall l w,
+  ~ Mem w (map fst l) ->
+  gather_keys_L w l = nil.
+induction l; intros; rew_map in *; simpl in *; auto.
+destruct a; case_if; simpl in *.
+elim H; apply Mem_here.
+rewrite IHl; auto; intro; elim H; rewrite Mem_cons_eq; right; auto.
+Qed.
+
+(* FIXME: do we really need all the 'locally closed' assumptions? *)
 Lemma L_to_Hyb_typing:
 forall Omega_L Gamma_L M_L A w_L G_Hyb Gamma_Hyb M_Hyb,
   L_to_Hyb_ctx Omega_L Gamma_L w_L = (G_Hyb, Some (w_L, Gamma_Hyb)) ->
   L_to_Hyb_term (fwo w_L) M_L M_Hyb ->
+  lc_w_L M_L -> lc_w_Hyb M_Hyb ->
   Omega_L; Gamma_L |- M_L ::: A @ w_L ->
   G_Hyb |= (w_L, Gamma_Hyb) |- M_Hyb ::: A.
 unfold L_to_Hyb_ctx; intros;
 generalize dependent G_Hyb;
 generalize dependent Gamma_Hyb;
 generalize dependent M_Hyb;
-induction H1; intros; inversion H0; subst; simpl in *.
+induction H3; intros; inversion H0; subst; simpl in *;
+inversion H1; inversion H2; subst.
 (* hyp *)
 constructor;
 [apply ok_L_to_Hyb_ctx_ok_Hyb with (Omega:=Omega) (Gamma:=Gamma) (w:=w)| ];
@@ -336,54 +478,197 @@ auto; eapply Mem_L_to_Hyb_ctx; eauto.
 apply t_lam_Hyb with (L:=L);
 [eapply ok_L_to_Hyb_ctx_ok_Hyb; eauto | intros]; unfold open_t_Hyb in *;
 unfold open_t_L in *; apply H with (x:=v'); auto.
+apply lc_w_subst_t_L; [constructor | ]; auto.
 apply L_to_Hyb_term_subst_t; simpl; auto.
-intros; constructor.
-destruct Ok;
-apply split_at_Hyb_cons; auto.
+constructor. intros; constructor.
+apply lc_w_subst_t_Hyb; [constructor | ]; auto.
+destruct Ok; apply split_at_Hyb_cons; auto.
 (* appl *)
 apply t_appl_Hyb with (A:=A);
 [eapply ok_L_to_Hyb_ctx_ok_Hyb |
  apply IHtypes_L1 | apply IHtypes_L2]; eauto.
 (* box *)
-apply t_box_Hyb with (L:=L0 \u L \u from_list (map fst_ Gamma)).
-eapply ok_Bg_Hyb_PPermut_Hyb with (y:= (w, Gamma_Hyb) :: G_Hyb);
-[PPermut_Hyb_simpl | eapply ok_L_to_Hyb_ctx_ok_Hyb; eauto].
+apply t_box_Hyb with (L:=L \u L0 \u
+                           from_list (map fst Gamma)).
+assert (G_Hyb & (w, Gamma_Hyb) ~=~ (w, Gamma_Hyb) :: G_Hyb) as HP
+  by PPermut_Hyb_simpl; rewrite HP;
+eapply ok_L_to_Hyb_ctx_ok_Hyb; eauto.
 intros; unfold open_w_L in *; unfold open_w_Hyb in *.
-assert (G_Hyb & (w, Gamma_Hyb) ~=~ bucket_sort_L Omega Gamma).
-apply permut_PPermut_Hyb;
-rewrite bucket_sort_L_permut with (w:=w) (Gamma':=Gamma_Hyb) (G:=G_Hyb);
-[permut_simpl | unfold L_to_Hyb_ctx; auto].
-rewrite H3. apply H; auto.
-apply L_to_Hyb_term_subst_w with (w:=w'); simpl; auto; case_if; auto.
-case_if.
-assert (gather_keys_L w' Gamma = nil).
-  skip. (* ! From w' freshness*)
-rewrite H5; auto.
+assert ( G_Hyb & (w, Gamma_Hyb) ~=~ bucket_sort_L Omega Gamma).
+  apply permut_PPermut_Hyb.
+  symmetry; rewrite bucket_sort_L_permut with
+            (w:=w) (Gamma':=Gamma_Hyb) (G:=G_Hyb); [permut_simpl | ]; auto.
+rewrite H5.
+eapply H; eauto. apply lc_w_subst_L; auto.
+apply L_to_Hyb_term_subst_w with (w:=fwo w').
+apply H6; eauto. case_if; auto.
+apply lc_w_subst_Hyb; auto.
+case_if; destruct Ok.
+rewrite gather_keys_L_fresh; [|apply notin_Mem]; eauto.
 (* unbox *)
 apply t_unbox_Hyb; auto;
 eapply ok_L_to_Hyb_ctx_ok_Hyb; eauto.
 (* fetch *)
-Focus 2.
+apply t_box_Hyb with (L:=used_w_vars_Hyb ((w', Gamma_Hyb) :: G_Hyb)).
+assert (G_Hyb & (w', Gamma_Hyb) ~=~ (w', Gamma_Hyb) :: G_Hyb)
+  by PPermut_Hyb_simpl; rewrite H4;
+eapply ok_L_to_Hyb_ctx_ok_Hyb; eauto.
+intros; unfold open_w_L in *; unfold open_w_Hyb in *; simpl;
+case_if.
+destruct (eq_var_dec w w'); subst.
+(* w = w' *)
+apply t_unbox_fetch_Hyb with (G:=G_Hyb) (Gamma:=Gamma_Hyb); auto.
+assert ((w', Gamma_Hyb) :: G_Hyb & (w'0, nil) ~=~
+        (w'0, nil) :: (w', Gamma_Hyb) :: G_Hyb) by PPermut_Hyb_simpl;
+rewrite H7; apply ok_Bg_Hyb_fresh_wo; [eapply ok_L_to_Hyb_ctx_ok_Hyb | ]; eauto.
+inversion H11; subst.
+assert (G_Hyb & (w'0, nil) ~=~ nil & (w'0, nil) ++ G_Hyb) by PPermut_Hyb_simpl.
+rewrite H7; apply GlobalWeakening_Hyb; rew_app.
+eapply IHtypes_L; auto.
+apply lc_w_n_shift_term_Sn_Hyb in H10;
+rewrite lc_w_shift_term_Hyb; auto;
+rewrite closed_subst_w_Hyb_bound with (n:=0); auto.
+apply lc_w_subst_Hyb; auto.
+assert ((w', Gamma_Hyb) :: (w'0, nil) :: G_Hyb ~=~
+        (w'0, nil) :: (w', Gamma_Hyb) :: G_Hyb) by PPermut_Hyb_simpl;
+rewrite H9. apply ok_Bg_Hyb_fresh_wo; auto;
+eapply ok_L_to_Hyb_ctx_ok_Hyb; eauto.
+(* w <> w' *)
+assert (exists G0, exists Gamma0,
+          split_at_Hyb (bucket_sort_L Omega Gamma) w = (G0, Some (w, Gamma0))).
+  exists (fst (split_at_Hyb (bucket_sort_L Omega Gamma) w)).
+  assert (exists Gamma1, snd (split_at_Hyb (bucket_sort_L Omega Gamma) w) =
+                 Some (w, Gamma1)).
+  apply L_to_Hyb_ctx_Mem_Some.
+  apply types_L_Mem_Omega in H3; auto.
+  destruct H7; exists x; rewrite <- H7; apply surjective_pairing.
+destruct H7 as (G0, (Gamma0, H7)).
+assert ((w, Gamma0) :: G0 *=* (w', Gamma_Hyb) :: G_Hyb).
+  transitivity (bucket_sort_L Omega Gamma); [symmetry | ];
+  apply bucket_sort_L_permut; eauto.
+apply t_unbox_fetch_Hyb with (G:=G0) (Gamma:=Gamma0).
+assert ((w, Gamma0) :: G0 & (w'0, nil) ~=~
+        (w'0, nil) :: (w, Gamma0) :: G0) by PPermut_Hyb_simpl.
+rewrite H10; apply ok_Bg_Hyb_fresh_wo; [eapply ok_L_to_Hyb_ctx_ok_Hyb | ];
+eauto. rewrite PPermut_Hyb_used_w with (y:=(w', Gamma_Hyb)::G_Hyb); auto;
+apply permut_PPermut_Hyb; auto.
+inversion H11; subst.
+assert (G0 & (w'0, nil) ~=~ nil & (w'0, nil) ++ G0) by PPermut_Hyb_simpl.
+rewrite H10; apply GlobalWeakening_Hyb; rew_app.
+eapply IHtypes_L; auto.
+apply lc_w_n_shift_term_Sn_Hyb in H13;
+rewrite lc_w_shift_term_Hyb; auto;
+rewrite closed_subst_w_Hyb_bound with (n:=0); auto.
+apply lc_w_subst_Hyb; auto.
+assert ((w, Gamma0) :: (w'0, nil) :: G0 ~=~
+        (w'0, nil) :: (w, Gamma0) :: G0) by PPermut_Hyb_simpl;
+rewrite H12. apply ok_Bg_Hyb_fresh_wo; auto.
+eapply ok_L_to_Hyb_ctx_ok_Hyb; eauto.
+rewrite PPermut_Hyb_used_w with (y:=(w', Gamma_Hyb)::G_Hyb); auto.
+apply permut_PPermut_Hyb; auto.
+apply permut_PPermut_Hyb;
+transitivity ((w, Gamma0)::G0); [| rewrite H9]; permut_simpl.
 (* here *)
 apply t_here_Hyb; auto;
 eapply ok_L_to_Hyb_ctx_ok_Hyb; eauto.
 (* get *)
-Focus 3.
-(* letd *)
-apply t_letdia_Hyb with (L_w:=Lw) (L_t:=Lt) (A:=A); auto.
+destruct (eq_var_dec w w'); subst.
+(* w = w' *)
+apply t_letdia_Hyb with (A:=A) (L_w:=used_w_vars_Hyb (G_Hyb & (w', Gamma_Hyb)))
+                               (L_t:=used_t_vars_Hyb (G_Hyb & (w', Gamma_Hyb))).
 eapply ok_L_to_Hyb_ctx_ok_Hyb; eauto.
-intros; unfold open_t_Hyb in *; unfold open_t_L in *;
-unfold open_w_Hyb in *; unfold open_w_L in *.
-apply H with (t:=v') (w':=w'); auto.
-apply  L_to_Hyb_term_subst_t.
-apply L_to_Hyb_term_subst_w with (w:=w).
-auto. case_if; auto. intros; constructor.
+eapply IHtypes_L; auto.
+intros; unfold open_t_Hyb; unfold open_w_Hyb; simpl; repeat case_if.
+apply t_get_here_Hyb with (G:=G_Hyb) (Gamma:=(v',A)::nil).
+apply ok_Bg_Hyb_fresh_wo_te; auto.
+assert (G_Hyb & (w', Gamma_Hyb) ~=~ (w', Gamma_Hyb) :: G_Hyb)
+  by PPermut_Hyb_simpl; rewrite H7;
+eapply ok_L_to_Hyb_ctx_ok_Hyb; eauto.
+constructor.
+apply ok_Bg_Hyb_fresh_wo_te; auto.
+assert (G_Hyb & (w', Gamma_Hyb) ~=~ (w', Gamma_Hyb) :: G_Hyb)
+  by PPermut_Hyb_simpl; rewrite H7;
+eapply ok_L_to_Hyb_ctx_ok_Hyb; eauto.
+apply Mem_here.
+PPermut_Hyb_simpl.
+(* w <> w' *)
+assert (exists G0, exists Gamma0,
+          split_at_Hyb (bucket_sort_L Omega Gamma) w = (G0, Some (w, Gamma0))).
+  exists (fst (split_at_Hyb (bucket_sort_L Omega Gamma) w)).
+  assert (exists Gamma1, snd (split_at_Hyb (bucket_sort_L Omega Gamma) w) =
+                 Some (w, Gamma1)).
+  apply L_to_Hyb_ctx_Mem_Some.
+  apply types_L_Mem_Omega in H3; auto.
+  destruct H7; exists x; rewrite <- H7; apply surjective_pairing.
+destruct H7 as (G0, (Gamma0, H7)).
+assert ((w, Gamma0) :: G0 *=* (w', Gamma_Hyb) :: G_Hyb).
+  transitivity (bucket_sort_L Omega Gamma); [symmetry | ];
+  apply bucket_sort_L_permut; eauto.
+apply t_unbox_fetch_Hyb with (G:=G0) (Gamma:=Gamma0).
+assert ((w, Gamma0) :: G0 & (w'0, nil) ~=~
+        (w'0, nil) :: (w, Gamma0) :: G0) by PPermut_Hyb_simpl.
+rewrite H10; apply ok_Bg_Hyb_fresh_wo; [eapply ok_L_to_Hyb_ctx_ok_Hyb | ];
+eauto. rewrite PPermut_Hyb_used_w with (y:=(w', Gamma_Hyb)::G_Hyb); auto;
+apply permut_PPermut_Hyb; auto.
+inversion H11; subst.
+assert (G0 & (w'0, nil) ~=~ nil & (w'0, nil) ++ G0) by PPermut_Hyb_simpl.
+rewrite H10; apply GlobalWeakening_Hyb; rew_app.
+eapply IHtypes_L; auto.
+apply lc_w_n_shift_term_Sn_Hyb in H13;
+rewrite lc_w_shift_term_Hyb; auto;
+rewrite closed_subst_w_Hyb_bound with (n:=0); auto.
+apply lc_w_subst_Hyb; auto.
+assert ((w, Gamma0) :: (w'0, nil) :: G0 ~=~
+        (w'0, nil) :: (w, Gamma0) :: G0) by PPermut_Hyb_simpl;
+rewrite H12. apply ok_Bg_Hyb_fresh_wo; auto.
+eapply ok_L_to_Hyb_ctx_ok_Hyb; eauto.
+rewrite PPermut_Hyb_used_w with (y:=(w', Gamma_Hyb)::G_Hyb); auto.
+apply permut_PPermut_Hyb; auto.
+apply permut_PPermut_Hyb;
+transitivity ((w, Gamma0)::G0); [| rewrite H9]; permut_simpl.
+
+(* letd *)
+apply t_letdia_Hyb with (L_w:=Lw \u from_list Omega \u from_list (map fst Gamma)
+                              \u used_w_vars_Hyb ((w, Gamma_Hyb) :: G_Hyb))
+                          (L_t:=Lt \u used_t_vars_Hyb ((w, Gamma_Hyb) :: G_Hyb))
+                          (A:=A); auto;
+[eapply ok_L_to_Hyb_ctx_ok_Hyb; eauto | intros];
+unfold open_w_L in *; unfold open_w_Hyb in *;
+unfold open_t_L in *; unfold open_t_Hyb in *.
+clear IHtypes_L HT2.
+assert (lc_w_L
+           (subst_t_L (hyp_L (fte v')) (bte 0)
+                      (subst_w_L N (fwo w') (bwo 0)))).
+  apply lc_w_subst_t_L; [ constructor | apply lc_w_subst_L]; auto.
+assert (G_Hyb & (w, Gamma_Hyb) ~=~ bucket_sort_L Omega Gamma).
+  apply permut_PPermut_Hyb.
+  symmetry; rewrite bucket_sort_L_permut with
+            (w:=w) (Gamma':=Gamma_Hyb) (G:=G_Hyb); [permut_simpl | ]; auto.
+eapply H; eauto. eauto. eauto.
+apply L_to_Hyb_term_subst_t; [ | constructor | intros; constructor ];
+apply L_to_Hyb_term_subst_w with (w:=fwo w); auto; case_if; auto.
+apply lc_w_subst_t_Hyb; [constructor | apply lc_w_subst_Hyb]; auto.
 repeat case_if.
+simpl in *; repeat rewrite notin_union in H6; destruct H6; destruct H13;
+destruct H14; destruct H16; rewrite notin_singleton in H16; elim H16; auto.
+rewrite bucket_sort_L_smaller; [| apply notin_Mem]; eauto;
+rewrite gather_keys_L_fresh; [| apply notin_Mem]; eauto;
+symmetry in H4; rewrite surjective_pairing in H4; inversion H4; subst;
+rewrite H18; auto.
+Qed
+              .
 
+Lemma L_to_Hyb_steps:
+forall M N w M',
+  L_to_Hyb_term w M N ->
+  steps_L (M, w) (M', w) ->
+  exists N', steps_Hyb (N, w) (N', w) /\ L_to_Hyb_term w M' N'.
+Admitted.
 
-
-
-
+Lemma L_to_Hyb_term_left_total:
+forall M w,
+  exists N, L_to_Hyb_term w M N.
+Admitted. (* problem for box *)
 
 Close Scope labeled_is5_scope.
 Close Scope permut_scope.
